ok

SStructTT/Defs/Syntax.lean
@@ -20,7 +20,7 @@ inductive Tm where
   | proj (A m n : Tm)
   | bool | tt | ff
   | ite  (A m n1 n2 : Tm)
-  | id   (A m n : Tm)
+  | idn  (A m n : Tm)
   | rfl  (m : Tm)
   | rw   (A h p : Tm)
 end Defs
@@ -46,7 +46,7 @@ def rename_rec (ξ : Var -> Var) (m : Tm Srt) : Tm Srt :=
   | tt => tt
   | ff => ff
   | ite A m n1 n2 => ite (rename_rec (upren ξ) A) (rename_rec ξ m) (rename_rec ξ n1) (rename_rec ξ n2)
-  | id A m n => id (rename_rec ξ A) (rename_rec ξ m) (rename_rec ξ n)
+  | idn A m n => idn (rename_rec ξ A) (rename_rec ξ m) (rename_rec ξ n)
   | rfl m => rfl (rename_rec ξ m)
   | rw A m n => rw (rename_rec (upren (upren ξ)) A) (rename_rec ξ m) (rename_rec ξ n)
 
@@ -67,8 +67,8 @@ variable (ξ : Var -> Var) (A B m n n1 n2 : Tm Srt) (x i : Nat) (r : Rlv) (s : S
 @[asimp]lemma bool : rename ξ (@bool Srt) = bool := by rfl
 @[asimp]lemma tt   : rename ξ (@tt Srt) = tt := by rfl
 @[asimp]lemma ff   : rename ξ (@ff Srt) = ff := by rfl
-@[asimp]lemma ite : rename ξ (ite A m n1 n2) = ite (rename (upren ξ) A) (rename ξ m) (rename ξ n1) (rename ξ n2) := by rfl
-@[asimp]lemma id   : rename ξ (id A m n) = id (rename ξ A) (rename ξ m) (rename ξ n) := by rfl
+@[asimp]lemma ite  : rename ξ (ite A m n1 n2) = ite (rename (upren ξ) A) (rename ξ m) (rename ξ n1) (rename ξ n2) := by rfl
+@[asimp]lemma idn  : rename ξ (idn A m n) = idn (rename ξ A) (rename ξ m) (rename ξ n) := by rfl
 @[asimp]lemma rfl  : rename ξ (rfl m) = rfl (rename ξ m) := by rfl
 @[asimp]lemma rw   : rename ξ (rw A m n) = rw (rename (upren $ upren ξ) A) (rename ξ m) (rename ξ n) := by rfl
 end Rename
@@ -87,7 +87,7 @@ def subst_rec (σ : Var -> Tm Srt) (m : Tm Srt) : Tm Srt :=
   | tt => tt
   | ff => ff
   | ite A m n1 n2 => ite (subst_rec (up σ) A) (subst_rec σ m) (subst_rec σ n1) (subst_rec σ n2)
-  | id A m n => id (subst_rec σ A) (subst_rec σ m) (subst_rec σ n)
+  | idn A m n => idn (subst_rec σ A) (subst_rec σ m) (subst_rec σ n)
   | rfl m => rfl (subst_rec σ m)
   | rw A m n => rw (subst_rec (upn 2 σ) A) (subst_rec σ m) (subst_rec σ n)
 
@@ -108,8 +108,8 @@ variable (σ : Var -> Tm Srt) (A B m n n1 n2 : Tm Srt) (x i : Nat) (r : Rlv) (s 
 @[asimp]lemma bool : subst σ (@bool Srt) = bool := by rfl
 @[asimp]lemma tt   : subst σ (@tt Srt) = tt := by rfl
 @[asimp]lemma ff   : subst σ (@ff Srt) = ff := by rfl
-@[asimp]lemma ite : subst σ (ite A m n1 n2) = ite (subst (up σ) A) (subst σ m) (subst σ n1) (subst σ n2) := by rfl
-@[asimp]lemma id   : subst σ (id A m n) = id (subst σ A) (subst σ m) (subst σ n) := by rfl
+@[asimp]lemma ite  : subst σ (ite A m n1 n2) = ite (subst (up σ) A) (subst σ m) (subst σ n1) (subst σ n2) := by rfl
+@[asimp]lemma idn  : subst σ (idn A m n) = idn (subst σ A) (subst σ m) (subst σ n) := by rfl
 @[asimp]lemma rfl  : subst σ (rfl m) = rfl (subst σ m) := by rfl
 @[asimp]lemma rw   : subst σ (rw A m n) = rw (subst (upn 2 σ) A) (subst σ m) (subst σ n) := by rfl
 end Subst
@@ -133,7 +133,7 @@ lemma rename_subst ξ (m : Tm Srt) : rename ξ m = m.[ren ξ] := by
   | tt => asimp
   | ff => asimp
   | ite A m n1 n2 ihA ihm ihn1 ihn2 => asimp[up_upren, ihA, ihm, ihn1, ihn2]
-  | id A m n ihA ihm ihn => asimp[ihA, ihm, ihn]
+  | idn A m n ihA ihm ihn => asimp[ihA, ihm, ihn]
   | rfl m ihm => asimp[ihm]
   | rw A m n ihA ihm ihn => asimp[up_upren, ihA, ihm, ihn]
 
@@ -157,7 +157,7 @@ lemma subst_id (m : Tm Srt) : m.[ids] = m := by
   | tt => asimp
   | ff => asimp
   | ite A m n1 n2 ihA ihm ihn1 ihn2 => asimp[up_ids, ihA, ihm, ihn1, ihn2]
-  | id A m n ihA ihm ihn => asimp[ihA, ihm, ihn]
+  | idn A m n ihA ihm ihn => asimp[ihA, ihm, ihn]
   | rfl m ihm => asimp[ihm]
   | rw A m n ihA ihm ihn => asimp[up_ids, ihA, ihm, ihn]
 
@@ -182,7 +182,7 @@ lemma ren_subst_comp ξ σ (m : Tm Srt) : m.[ren ξ].[σ] = m.[ξ !>> σ] := by
   | tt => asimp
   | ff => asimp
   | ite A m n1 n2 ihA ihm ihn1 ihn2 => asimp[up_upren, up_comp_upren, ihA, ihm, ihn1, ihn2]
-  | id A m n ihA ihm ihn => asimp[ihA, ihm, ihn]
+  | idn A m n ihA ihm ihn => asimp[ihA, ihm, ihn]
   | rfl m ihm => asimp[ihm]
   | rw A m n ihA ihm ihn => asimp[up_upren, up_comp_upren, ihA, ihm, ihn]
 
@@ -211,7 +211,7 @@ lemma subst_ren_comp σ ξ (m : Tm Srt) : m.[σ].[ren ξ] = m.[σ !>> rename ξ]
   | tt => asimp
   | ff => asimp
   | ite A m n1 n2 ihA ihm ihn1 ihn2 => asimp[up_upren, up_comp_ren, ihA, ihm, ihn1, ihn2]
-  | id A m n ihA ihm ihn => asimp[ihA, ihm, ihn]
+  | idn A m n ihA ihm ihn => asimp[ihA, ihm, ihn]
   | rfl m ihm => asimp[ihm]
   | rw A m n ihA ihm ihn => asimp[up_upren, up_comp_ren, ihA, ihm, ihn]
 
@@ -240,7 +240,7 @@ lemma subst_comp (σ τ : Var -> Tm Srt) m : m.[σ].[τ] = m.[σ !> τ] := by
   | tt => asimp
   | ff => asimp
   | ite A m n1 n2 ihA ihm ihn1 ihn2 => asimp[up_comp, ihA, ihm, ihn1, ihn2]
-  | id A m n ihA ihm ihn => asimp[ihA, ihm, ihn]
+  | idn A m n ihA ihm ihn => asimp[ihA, ihm, ihn]
   | rfl m ihm => asimp[ihm]
   | rw A m n ihA ihm ihn => asimp[up_comp, ihA, ihm, ihn]
 
